rich_raven_lang/trnsl.v
@@ -18,33 +18,7 @@ From iris.program_logic Require Import ectx_lifting.
 From raven_iris.simp_raven_lang Require Import lang lifting ghost_state.
 From raven_iris.rich_raven_lang Require Import rrl_lang.
 
-
-(* Context `{!simpLangG Σ}. *)
-
-
 Section MainTranslation.
-    (* Context `{!simpLangG Σ}. *)
-  
-    Program Fixpoint trnsl_atomic_annotation (mask: coPset) (a : AtomicAnnotation) {measure match a.2 with | Closed => 0 | Opened s => length s | Stepped s => length s end} : iProp rrl_lang.Σ :=
-      match a.2 with
-      | Closed => True
-      | Opened [] => False
-      | Stepped [] => False
-      | Opened (inv :: invs) => True ∗ trnsl_atomic_annotation (mask ∪ ↑(inv_namespace_map inv.1)) (a.1, Opened invs)
-  
-      | Stepped (inv :: invs) => True ∗ trnsl_atomic_annotation (mask ∪ ↑(inv_namespace_map inv.1)) (a.1, Stepped invs)
-      end
-      .
-      Next Obligation.
-      intros. simpl; subst filtered_var; rewrite <- Heq_anonymous. simpl; lia.
-      Qed.
-      Next Obligation.
-      intros. simpl; subst filtered_var; rewrite <- Heq_anonymous. simpl; lia.
-      Qed.
-      Next Obligation.
-      intros. simpl. Admitted.
-  
-  
     Definition inv_set_to_namespace (s : gset inv_name) : coPset :=
       set_fold (λ inv acc, acc ∪ ↑(inv_namespace_map inv)) ∅ s.
 
@@ -63,20 +37,20 @@ Section MainTranslation.
       interp_lexpr lexpr mp = Some lv.
     Admitted.
 
-    Definition trnsl_hoare_triple (stk_id: stack_id) (p : assertion) (msk : maskAnnot) (cmd : stmt) (q : assertion) (mp : symb_map) : iProp rrl_lang.Σ :=
+    Definition trnsl_hoare_triple Γ (stk_id: stack_id) (p : assertion) (msk : maskAnnot) (cmd : stmt) (q : assertion) (mp : symb_map) : iProp rrl_lang.Σ :=
         match (trnsl_stmt cmd) with 
         | Error => True
         | None' =>
-          match (trnsl_assertion p stk_id mp), 
-                (trnsl_assertion q stk_id mp) with
+          match (trnsl_assertion Γ p stk_id mp), 
+                (trnsl_assertion Γ q stk_id mp) with
           | None, _ | _, None => True
           | Some p', Some q' =>
             p'={inv_set_to_namespace msk}=∗ q'
           end
         
         | Some' s =>
-          match (trnsl_assertion p stk_id mp), 
-                (trnsl_assertion q stk_id mp) with
+          match (trnsl_assertion Γ p stk_id mp), 
+                (trnsl_assertion Γ q stk_id mp) with
           | None, _ | _, None => True
           | Some p', Some q' => 
             {{{ p' }}}  
@@ -105,8 +79,6 @@ Section MainTranslation.
       - apply internal_val_dec_bl in Hvb. done.
       - inversion H1.
     Qed.
-
-
 
     Lemma val_beq_refl (v : val) : val_beq v v = true.
     Proof.
@@ -189,9 +161,8 @@ Section MainTranslation.
           rewrite HstkI. simpl. done.
     Qed.
 
-
     Axiom proc_specs_valid :
-      forall proc proc_record stk_vals, 
+      forall Γ proc proc_record stk_vals, 
       proc ∈ proc_set  ->
       proc_map !! proc = Some proc_record ->
 
@@ -202,25 +173,26 @@ Section MainTranslation.
 
       Forall2 (λ var val, stk_frm.(locals) !! var = Some val) (proc_args_of proc_record).*1 stk_vals ->
 
-      
-
       let subst_map' := list_to_map (zip (proc_args_of proc_record).*1 (map (λ val, LVal (trnsl_val val)) stk_vals)) in
 
-
-      trnsl_assertion (subst (proc_precond_of proc_record) subst_map') stk_id mp = Some precond ->
-      trnsl_assertion (subst (proc_postcond_of proc_record) (<["#ret_val" := LVal (trnsl_val (ret_val))]> subst_map')) stk_id mp = Some postcond ->
+      trnsl_assertion Γ (subst (proc_precond_of proc_record) subst_map') stk_id mp = Some precond ->
+      trnsl_assertion Γ (subst (proc_postcond_of proc_record) (<["#ret_val" := LVal (trnsl_val (ret_val))]> subst_map')) stk_id mp = Some postcond ->
       
       ((trnsl_stmt (proc_body_of proc_record) = Some' stmt) \/ (trnsl_stmt (proc_body_of proc_record) = None' /\ stmt = lang.SkipS) ) ->
       (∃ stk_frm'',
       ({{{ stack_own[stk_id, stk_frm] ∗ precond }}} (to_rtstmt stk_id stmt) @ mask {{{ RET lang.LitUnit; stack_own[stk_id, stk_frm''] ∗ ⌜ (locals stk_frm'' !! "#ret_val") = Some ret_val ⌝ ∗ postcond }}})).
 
-    
+    (* Lemma transport_congr {A B : cmra} (H : (cmra_car A) = (cmra_car B)) {x y : A} (Hupd : x ~~> y) :
+      transport H x ~~> transport H y.
+    Proof.
+      unfold transport. revert Hupd.
+    (* usually trivial by proper instance or f_equiv *) Admitted. *)
 
-    Theorem rrl_validity ρ σ stk_id p msk cmd q :
+    Theorem rrl_validity Γ ρ σ stk_id p msk cmd q :
       stmt_well_defined ρ cmd -> 
       forall mp, (env_typ_well_defined σ mp) ->
        ⌜RavenHoareTriple ρ σ p cmd msk q⌝
-      ⊢  (trnsl_hoare_triple stk_id p msk cmd q mp).
+      ⊢  (trnsl_hoare_triple Γ stk_id p msk cmd q mp).
     Proof.
       iIntros (Hwelldef mp Henv) "%H". 
       iInduction H as 
@@ -237,19 +209,17 @@ Section MainTranslation.
         { inversion Ht. } 
 
         inversion Ht. simpl. 
-        (* destruct (trnsl_lval old_val); destruct (trnsl_lval new_val); simpl; iIntros; try done. *)
         - iIntros (Φ). iModIntro.
-        iIntros "[Hstk1 Hstk2] HΦ".
+          iIntros "[Hstk1 Hstk2] HΦ".
 
-        iDestruct "Hstk2" as "[%l [%Hlexpr1 Hlfld]]".
-        
-        iApply (wp_heap_wr stk_id (symb_stk_to_stk_frm stk mp) _ _ _ l _ _ _ with "[Hstk1 Hlfld]").
+          iDestruct "Hstk2" as "[%l [%Hlexpr1 Hlfld]]".
+          
+          iApply (wp_heap_wr stk_id (symb_stk_to_stk_frm stk mp) _ _ _ l _ _ _ with "[Hstk1 Hlfld]").
         
         {
           iFrame.
           iSplit.
           { iPureIntro. simpl. rewrite lookup_fmap. 
-            (* rewrite HLexpr. simpl. apply f_equal.  *)
             rewrite Hatm. simpl. unfold LExpr_holds in Hlexpr1. simpl in Hlexpr1. injection Hlexpr1 as Hlv. 
             destruct (val_beq (mp lv) (LitLoc l)) eqn:Hlv'.
             - apply f_equal.
@@ -276,9 +246,9 @@ Section MainTranslation.
         (* INV ACCESS BLOCK *)
         unfold trnsl_hoare_triple.
 
-        pose proof (trnsl_inv_validity invr lexprs stk_id mp) as Htrnsl_inv_valid.
+        pose proof (trnsl_inv_validity Γ invr lexprs stk_id mp) as Htrnsl_inv_valid.
         rewrite Hinv_record in Htrnsl_inv_valid. simpl in Htrnsl_inv_valid.
-        destruct (trnsl_assertion (rrl_lang.subst (inv_body inv_record)
+        destruct (trnsl_assertion Γ (rrl_lang.subst (inv_body inv_record)
         subst) stk_id mp) eqn:HinvBody. 2:{ rewrite HinvBody in Htrnsl_inv_valid. inversion Htrnsl_inv_valid. }
 
         rewrite HinvBody in Htrnsl_inv_valid. injection Htrnsl_inv_valid as Htrnsl_inv.
@@ -288,11 +258,11 @@ Section MainTranslation.
 
         
         { 
-          destruct (trnsl_assertion (LStack stk) stk_id mp) eqn:Hstack.
+          destruct (trnsl_assertion Γ (LStack stk) stk_id mp) eqn:Hstack.
           2 : { simpl in Hstack. inversion Hstack. }
 
           simpl. rewrite HinvBody. rewrite Hinv_record.
-           destruct (trnsl_assertion p stk_id mp) eqn:Hp, (trnsl_assertion q stk_id mp) eqn:Hq; try done.
+           destruct (trnsl_assertion Γ p stk_id mp) eqn:Hp, (trnsl_assertion Γ q stk_id mp) eqn:Hq; try done.
            
            iIntros "[Hstk [#H Hu]]".
            (* unfold trnsl_hoare_triple in IH. *)
@@ -311,9 +281,6 @@ Section MainTranslation.
           iDestruct "Hinv" as ">Hinv".
           iCombine "Hstk Hinv Hu" as "Hcomb".
           inversion Hwelldef as [ | | | | | | | | | | | | | inv args' stmt' HInvSet HargsWellDef HBodywelldef | ]; subst stmt' args'.
-          (* iCombine "Hcomb1 Hstk" as "Hcomb2". *)
-          (* Unset Printing Notations. *)
-          (* iPoseProof IHHbody as "Htriple". *)
           
           iPoseProof ("IH" with  "[%] [%] Hcomb") as "IH2"; try done.
           iFrame.
@@ -332,7 +299,7 @@ Section MainTranslation.
           simpl.
           iEval (rewrite H HinvBody) in "IH" .
           iEval (rewrite Hinv_record).
-          destruct (trnsl_assertion p stk_id mp) eqn:Hp, (trnsl_assertion q stk_id mp) eqn:Hq; try done.
+          destruct (trnsl_assertion Γ p stk_id mp) eqn:Hp, (trnsl_assertion Γ q stk_id mp) eqn:Hq; try done.
           iIntros (Φ).
           iModIntro.
           iIntros "[Hstk [#HInv Hu]] HΦ".
@@ -381,7 +348,6 @@ Section MainTranslation.
             iFrame.
             iPureIntro.
             apply (trnsl_expr_interp_lexpr_compatibility _ _ lexpr). { done. } 
-
             done. 
           }
           
@@ -423,7 +389,7 @@ Section MainTranslation.
         }
 
         pose proof (expr_interp_well_defined stk e mp lexpr H Hlexpr).
-        inversion Hwelldef as [ | | | | | | | | | | | | | inv args' stmt' HInvSet HargsWellDef HBodywelldef | ].
+        inversion Hwelldef.
         contradiction.
       }
 
@@ -435,19 +401,22 @@ Section MainTranslation.
         unfold trnsl_hoare_triple. simpl.
         destruct (trnsl_stmt s) eqn:Htrnsl; try done.
         { simpl.
-          destruct (trnsl_assertion p stk_id mp) eqn:Hp, (trnsl_assertion q stk_id mp) eqn:Hq, (trnsl_assertion r stk_id mp) eqn:Hr; try done. 
+          destruct (trnsl_assertion Γ p stk_id mp) eqn:Hp, (trnsl_assertion Γ q stk_id mp) eqn:Hq, (trnsl_assertion Γ r stk_id mp) eqn:Hr; try done. 
 
           iIntros "[Hu Hu1]".
           iPoseProof ("IH2" with "[%] Hu") as ">IH3"; try done. iModIntro; iFrame.
 
         }
 
-        { destruct (trnsl_assertion p stk_id mp) eqn:Hp, (trnsl_assertion q stk_id mp) eqn:Hq, (trnsl_assertion r stk_id mp) eqn:Hr; try done.  
-        
-        iIntros (Φ).
-        iModIntro. iIntros "[Hu Hu1] HΦ".
-        iApply ("IH2" with "[%] Hu"); try done.
-        iNext. iIntros "Hu0". iApply "HΦ". iFrame.
+        { 
+          destruct (trnsl_assertion Γ p stk_id mp) eqn:Hp, 
+                   (trnsl_assertion Γ q stk_id mp) eqn:Hq, 
+                   (trnsl_assertion Γ r stk_id mp) eqn:Hr; try done.
+
+          iIntros (Φ).
+          iModIntro. iIntros "[Hu Hu1] HΦ".
+          iApply ("IH2" with "[%] Hu"); try done.
+          iNext. iIntros "Hu0". iApply "HΦ". iFrame.
         }
       }
 
@@ -463,12 +432,9 @@ Section MainTranslation.
           inversion Hwelldef. contradiction.
         }
 
-        pose proof (lexpr_holds_interp_compat _ _ _ _ HLe_h Hinterp) .
-          subst v.
+        pose proof (lexpr_holds_interp_compat _ _ _ _ HLe_h Hinterp). subst v.
 
         iApply (wp_heap_rd stk_id (rrl_lang.symb_stk_to_stk_frm stk mp) fld e (trnsl_lval val) l x _ 1%Qp with "[Hstk H_l_hp]").
-
-        
 
         {
           pose proof (trnsl_expr_interp_lexpr_compatibility _ _ _ _ _ H Hinterp).
@@ -487,16 +453,15 @@ Section MainTranslation.
           iExists val.
 
           iSplitL "Hstk".
-          - pose proof 
-          (fresh_mp_rewrite_symb_stk_to_stk_frm_compat stk lvar_x x mp val H0) as HstkOwnDone.
-          rewrite HstkOwnDone. iFrame.
+          - pose proof (fresh_mp_rewrite_symb_stk_to_stk_frm_compat stk lvar_x x mp val H0) as HstkOwnDone.
+            rewrite HstkOwnDone. iFrame.
 
           - iSplitL.
             + iExists l. 
-            iFrame; iPureIntro.
-            pose proof (fresh_var_trnsl_expr_invariant stk lvar_x e _ mp val H0 H).
-            unfold LExpr_holds.
-            simpl. rewrite <- H2. apply HLe_h.
+              iFrame; iPureIntro.
+              pose proof (fresh_var_trnsl_expr_invariant stk lvar_x e _ mp val H0 H).
+              unfold LExpr_holds.
+              simpl. rewrite <- H2. apply HLe_h.
           
             + iPureIntro. unfold LExpr_holds. simpl. rewrite String.eqb_refl. rewrite val_beq_refl. done.
         }
@@ -527,42 +492,37 @@ Section MainTranslation.
 
           + simpl. destruct a as [fld val].
           assert (stmt_well_defined ρ (Alloc x fld_vals)) as Hwell_def'. { admit. }
-          destruct (trnsl_assertion (field_list_to_assertion (LVar lvar_x) fld_vals) stk_id mp' ) eqn:Htrfl.
+          destruct (trnsl_assertion Γ (field_list_to_assertion (LVar lvar_x) fld_vals) stk_id mp' ) eqn:Htrfl.
           
             * simpl. rewrite Htrfl.
-            iPoseProof ("IH" with "[%]") as "IH2"; try done.
-            iClear "IH".
-            iDestruct "Hhp" as "[Hhpl Hhpfvs]".
-            iPoseProof ("IH2" with "Hstk Hhpfvs") as "[IH3 IH3']". 
-            iFrame. iExists l. 
-            assert (trnsl_lval (trnsl_val val) = val) as H1. { admit. } 
-            rewrite H1. iFrame.
-            iPureIntro. 
-            unfold LExpr_holds.
-            simpl.
-            subst mp'. simpl. rewrite String.eqb_refl. rewrite val_beq_refl. done.
+              iPoseProof ("IH" with "[%]") as "IH2"; try done.
+              iClear "IH".
+              iDestruct "Hhp" as "[Hhpl Hhpfvs]".
+              iPoseProof ("IH2" with "Hstk Hhpfvs") as "[IH3 IH3']". 
+              iFrame. iExists l. 
+              assert (trnsl_lval (trnsl_val val) = val) as H1. { admit. } 
+              rewrite H1. iFrame.
+              iPureIntro. 
+              unfold LExpr_holds.
+              simpl.
+              subst mp'. simpl. rewrite String.eqb_refl. rewrite val_beq_refl. done.
 
             * simpl. rewrite Htrfl. iPoseProof ("IH" with "[%]") as "IH2"; try done.
-             (* iClear "IH".
-            iDestruct "Hhp" as "[Hhpl Hhp2]". 
-            iApply ("IH2" with "Hstk Hhp2").   *)
       }
-
 
       4 : {
         (* UNFOLD PRED *)
         unfold trnsl_hoare_triple.
         simpl.
-        pose proof (trnsl_pred_validity pred lexprs stk_id mp) as HPredTrnsl. rewrite H0 in HPredTrnsl. unfold subst_map in HPredTrnsl. rewrite HPredTrnsl.
+        pose proof (trnsl_pred_validity Γ pred lexprs stk_id mp) as HPredTrnsl. rewrite H0 in HPredTrnsl. unfold subst_map in HPredTrnsl. rewrite HPredTrnsl.
         iIntros. iModIntro.  iFrame.
-
       }
 
       4 : {
         (* FOLD PRED *)
         unfold trnsl_hoare_triple.
         simpl.
-        pose proof (trnsl_pred_validity pred lexprs stk_id mp) as HPredTrnsl. rewrite H1 in HPredTrnsl. unfold subst_map in HPredTrnsl. rewrite HPredTrnsl.
+        pose proof (trnsl_pred_validity Γ pred lexprs stk_id mp) as HPredTrnsl. rewrite H1 in HPredTrnsl. unfold subst_map in HPredTrnsl. rewrite HPredTrnsl.
         iIntros. iModIntro.  iFrame.
       }
 
@@ -575,25 +535,24 @@ Section MainTranslation.
 
         unfold trnsl_hoare_triple. 
         simpl.
-        destruct (trnsl_assertion a2 stk_id mp) eqn:Ha2.
+        destruct (trnsl_assertion Γ a2 stk_id mp) eqn:Ha2.
         - destruct (trnsl_stmt c1) eqn:Hc1, (trnsl_stmt c2) eqn:Hc2; try done.
-          + destruct (trnsl_assertion a1 stk_id mp) eqn:Ha1, (trnsl_assertion a3 stk_id mp) eqn: Ha3; try done. iIntros "Hu0".
+          + destruct (trnsl_assertion Γ a1 stk_id mp) eqn:Ha1, (trnsl_assertion Γ a3 stk_id mp) eqn: Ha3; try done. iIntros "Hu0".
           iPoseProof ("IH'" with "[%] Hu0") as ">IHH"; try done.
            iApply "IH1'"; try done.
 
-          + destruct (trnsl_assertion a1 stk_id mp) eqn:Ha1, (trnsl_assertion a3 stk_id mp) eqn: Ha3; try done. 
+          + destruct (trnsl_assertion Γ a1 stk_id mp) eqn:Ha1, (trnsl_assertion Γ a3 stk_id mp) eqn: Ha3; try done. 
             iIntros (Φ). iModIntro. iIntros "Hu0 HΦ".
             iPoseProof ("IH'" with "[%] Hu0") as ">IHH"; try done.
             iApply ("IH1'" with "[%] IHH"); try done.
 
-          + destruct (trnsl_assertion a1 stk_id mp) eqn:Ha1, (trnsl_assertion a3 stk_id mp) eqn: Ha3; try done. admit.
+          + destruct (trnsl_assertion Γ a1 stk_id mp) eqn:Ha1, (trnsl_assertion Γ a3 stk_id mp) eqn: Ha3; try done. admit.
 
-          + destruct (trnsl_assertion a1 stk_id mp) eqn:Ha1, (trnsl_assertion a3 stk_id mp) eqn: Ha3; try done.
+          + destruct (trnsl_assertion Γ a1 stk_id mp) eqn:Ha1, (trnsl_assertion Γ a3 stk_id mp) eqn: Ha3; try done.
           simpl.
           iApply wp_seq.
             { iApply "IH'"; try done. }
             { iApply "IH1'"; try done. }
-
 
         - admit.
            (* Case: trnsl_assertion a2 = None; *)
@@ -603,9 +562,7 @@ Section MainTranslation.
       5 : {
         (* SKIP *)
         unfold trnsl_hoare_triple. simpl.
-        destruct (trnsl_assertion p stk_id mp); try done.
-        (* Unset Printing Notations. *)
-        (* iApply (wp_skip (stack_own[ stk_id, symb_stk_to_stk_frm stk mp] ∗ u ) (inv_set_to_namespace mask) (stk_id)). *)
+        destruct (trnsl_assertion Γ p stk_id mp); try done.
         iIntros (Φ). iModIntro. iIntros "Hp HΦ".
         iApply (wp_skip with "Hp"). iFrame. 
       }
@@ -631,7 +588,6 @@ Section MainTranslation.
         apply val_beq_eq in Hv0_l. rewrite Hv0_l in Hlexpr1.
         
         pose proof (trnsl_expr_interp_lexpr_compatibility _ _ _ _ _ H0 Hlexpr1) as Hexpr_step_e1.
-
 
         iApply (wp_cas_succ v e1 fld e2 e3 stk_id (symb_stk_to_stk_frm stk mp) l (trnsl_lval old_val) (trnsl_lval new_val) with "[Hstk Hl]"); try done.
         
@@ -661,18 +617,15 @@ Section MainTranslation.
 
          iPureIntro.
          unfold LExpr_holds. simpl. rewrite String.eqb_refl. rewrite val_beq_refl. done.
-
       }
 
       5 : {
-        (* CASS FAIL *)
+        (* CAS FAIL *)
         unfold trnsl_hoare_triple; simpl.
         iIntros (Φ). iModIntro. iIntros "[Hstk [He1 %Hneq]] HΦ".
         iDestruct "He1" as (l) "[%He1 Hl]".
         assert (interp_lexpr (LVal old_val2) mp = Some old_val2) as Hinterp_old; try done.
-        (* assert (interp_lexpr (LVal old_val) mp = Some new_val) as Hinterp_new; try done. *)
         pose proof (trnsl_expr_interp_lexpr_compatibility _ _ _ _ _ H1 Hinterp_old) as Hexpr_step_e2.
-        (* pose proof (trnsl_expr_interp_lexpr_compatibility _ _ _ _ _ H2 Hinterp_new) as Hexpr_step_e3. *)
         unfold LExpr_holds in He1. simpl in He1.
         destruct (interp_lexpr lexpr1 mp) eqn:Hlexpr1.
         2 : { 
@@ -722,19 +675,17 @@ Section MainTranslation.
           { 
             iPureIntro. unfold LExpr_holds; simpl.
             apply f_equal. rewrite String.eqb_refl. rewrite val_beq_refl. done.
-
           }
-
       }
 
       4 : {
         (* WEAKENING *)
         unfold entails in *.
         unfold trnsl_hoare_triple. simpl.
-        specialize H0 with stk_id mp.
+        specialize H0 with Γ stk_id mp.
         destruct H0 as [P' [P [HP' [HP HP_ent_P']]]].
         
-        specialize H1 with stk_id mp.
+        specialize H1 with Γ stk_id mp.
         destruct H1 as [Q [Q' [HQ [HQ' HQ_ent_Q']]]].
         rewrite HP HP' HQ HQ'.
 
@@ -772,8 +723,7 @@ Section MainTranslation.
           unfold trnsl_lval in Hle_val. destruct (val0) eqn: Hle_val'; try done.
 
         destruct (trnsl_stmt s1) eqn:Hs1, (trnsl_stmt s2) eqn:Hs2; try done;
-
-        destruct (trnsl_assertion p stk_id mp) eqn:HP, (trnsl_assertion q stk_id mp) eqn:HQ; try done.
+        destruct (trnsl_assertion Γ p stk_id mp) eqn:HP, (trnsl_assertion Γ q stk_id mp) eqn:HQ; try done.
 
         - destruct b0.
 
@@ -795,8 +745,6 @@ Section MainTranslation.
             iPoseProof ("IH'" with "[%] [Hstk Hu]" ) as "HQ"; try done; try iFrame.
             { iPureIntro. unfold LExpr_holds. rewrite Hinterp_lexpr. done.  }
             iMod "HQ". iApply (wp_skip (stack_own[ stk_id, symb_stk_to_stk_frm stk2 mp] ∗ u0) with "[HQ]"); iFrame.
-
-            
           
           + iApply (wp_if_f e (RTSkipS stk_id) (to_rtstmt stk_id s) stk_id (symb_stk_to_stk_frm stk1 mp) u (stack_own[ stk_id, symb_stk_to_stk_frm stk2 mp] ∗ u0) (lang.LitUnit) (inv_set_to_namespace mask) with "[IH'] [IH' Hstk Hu ] [HΦ]"); try iFrame.
             * apply (trnsl_expr_interp_lexpr_compatibility _ e lexpr (LitBool false) mp); try done.
@@ -805,7 +753,6 @@ Section MainTranslation.
             iPoseProof ("IH1'" with "[%] [Hstk Hu]" ) as "HQ"; try done; try iFrame.
             { iPureIntro. unfold LExpr_holds. simpl. rewrite Hinterp_lexpr. done.  }
             iApply "HQ"; iFrame.
-            
 
         - iIntros (Φ). iModIntro. iIntros "[Hstk Hu] HΦ".
           destruct b0.
@@ -816,9 +763,6 @@ Section MainTranslation.
             iPoseProof ("IH'" with "[%] [Hstk Hu]" ) as "HQ"; try done; try iFrame.
             { iPureIntro. unfold LExpr_holds. rewrite Hinterp_lexpr. done.  }
             iApply "HQ"; iFrame.
-            
-
-            
           
           + iApply (wp_if_f e (to_rtstmt stk_id s) (RTSkipS stk_id) stk_id (symb_stk_to_stk_frm stk1 mp) u (stack_own[ stk_id, symb_stk_to_stk_frm stk2 mp] ∗ u0) (lang.LitUnit) (inv_set_to_namespace mask) with "[IH'] [IH' Hstk Hu ] [HΦ]"); try iFrame.
             * apply (trnsl_expr_interp_lexpr_compatibility _ e lexpr (LitBool false) mp); try done.
@@ -838,9 +782,6 @@ Section MainTranslation.
             { iPureIntro. unfold LExpr_holds. rewrite Hinterp_lexpr. done.  }
             iApply "HQ"; iFrame.
             
-
-            
-          
           + iApply (wp_if_f e (to_rtstmt stk_id s) (to_rtstmt stk_id s0) stk_id (symb_stk_to_stk_frm stk1 mp) u (stack_own[ stk_id, symb_stk_to_stk_frm stk2 mp] ∗ u0) (lang.LitUnit) (inv_set_to_namespace mask) with "[IH'] [IH' Hstk Hu ] [HΦ]"); try iFrame.
             * apply (trnsl_expr_interp_lexpr_compatibility _ e lexpr (LitBool false) mp); try done.
 
@@ -859,9 +800,9 @@ Section MainTranslation.
         pose proof H0 as Hspec_StackFree.
         apply proc_spec_stack_free in Hspec_StackFree.
 
-        destruct (trnsl_assertion (LAnd (LStack stk) (LAnd (LProc proc_name proc_record) (subst (proc_precond_of proc_record) subst_map))) stk_id mp) eqn:HPreCond; try done.
+        destruct (trnsl_assertion Γ (LAnd (LStack stk) (LAnd (LProc proc_name proc_record) (subst (proc_precond_of proc_record) subst_map))) stk_id mp) eqn:HPreCond; try done.
 
-        destruct (trnsl_assertion
+        destruct (trnsl_assertion Γ
           (LExists lvar_x
           (LAnd (LStack (<[x:=lvar_x]> stk))
           (subst (proc_postcond_of proc_record) (<["#ret_var":=LVar lvar_x]> subst_map)))) stk_id mp
@@ -915,7 +856,7 @@ Section MainTranslation.
 
         simpl in *.
         destruct proc_record as [proc_args proc_locals proc_pre proc_post proc_body] eqn:Hproc_record.
-        destruct (trnsl_stmt (proc_body)) eqn:Hproc_body, (trnsl_assertion (subst proc_pre subst_map) stk_id mp) eqn:Hproc_pre; try rewrite Hproc_pre in HPreCond;  try discriminate; simpl in HPreCond.
+        destruct (trnsl_stmt (proc_body)) eqn:Hproc_body, (trnsl_assertion Γ (subst proc_pre subst_map) stk_id mp) eqn:Hproc_pre; try rewrite Hproc_pre in HPreCond;  try discriminate; simpl in HPreCond.
         
         {   
           (* proc_body = Skip *)
@@ -925,22 +866,18 @@ Section MainTranslation.
         
         iIntros "[Hstk [Hproc_tbl Hu1]] HΦ".
 
-        (* pose proof (proc_specs_valid proc_name (Proc proc_args proc_locals proc_pre proc_post proc_body) u1 u0 stk_id' mp lang.SkipS (inv_set_to_namespace mask) stk_frm' arg_vals) as [ret_val Hproc]. *)
-
-        (* destruct HPostCond' as [ret_val HPostCond]. *)
-
-        pose proof (proc_specs_valid proc_name (Proc proc_args proc_locals proc_pre proc_post proc_body) arg_vals ) as [ret_val Hproc]; try done.
+        pose proof (proc_specs_valid Γ proc_name (Proc proc_args proc_locals proc_pre proc_post proc_body) arg_vals ) as [ret_val Hproc]; try done.
 
         set (subst_map' := @list_to_map var LExpr (gmap var LExpr) _ _ (zip (proc_args).*1 (map (λ val, LVal (trnsl_val val)) arg_vals))).
 
-          destruct (trnsl_assertion (subst proc_pre subst_map') stk_id mp) as [ proc_frame_pre |] eqn: Hproc_frame_pre.
+          destruct (trnsl_assertion Γ (subst proc_pre subst_map') stk_id mp) as [ proc_frame_pre |] eqn: Hproc_frame_pre.
           
           2 : {  
             (* trnsl_assertion (subst proc_pre subst_map') stk_id' mp CANNOT BE None *)
             admit.
           }
 
-          destruct (trnsl_assertion (subst proc_post (<["#ret_val":=LVal (trnsl_val ret_val)]> subst_map')) stk_id mp) as [ proc_frame_post |] eqn: Hproc_frame_post.
+          destruct (trnsl_assertion Γ (subst proc_post (<["#ret_val":=LVal (trnsl_val ret_val)]> subst_map')) stk_id mp) as [ proc_frame_post |] eqn: Hproc_frame_post.
 
           2 : {
             (* trnsl_assertion (subst proc_pre subst_map') stk_id' mp CANNOT BE None *)
@@ -969,9 +906,9 @@ Section MainTranslation.
 
           simpl in HlocalsDef. pose proof (Hproc HlocalsDef) as Hproc.
 
-          rewrite (stack_free_assertion_trnsl (subst proc_pre subst_map') stk_id stk_id' mp) in Hproc_frame_pre. 2 : { apply stack_free_assertion_subst. destruct Hspec_StackFree; done. }
+          rewrite (stack_free_assertion_trnsl Γ (subst proc_pre subst_map') stk_id stk_id' mp) in Hproc_frame_pre. 2 : { apply stack_free_assertion_subst. destruct Hspec_StackFree; done. }
 
-          rewrite (stack_free_assertion_trnsl (subst proc_post (<["#ret_val":=LVal (trnsl_val ret_val)]> subst_map')) stk_id stk_id' mp) in Hproc_frame_post. 2 : { apply stack_free_assertion_subst. destruct Hspec_StackFree; done. }
+          rewrite (stack_free_assertion_trnsl Γ (subst proc_post (<["#ret_val":=LVal (trnsl_val ret_val)]> subst_map')) stk_id stk_id' mp) in Hproc_frame_post. 2 : { apply stack_free_assertion_subst. destruct Hspec_StackFree; done. }
 
           pose proof (Hproc Hproc_frame_pre Hproc_frame_post) as Hproc.
 
@@ -990,38 +927,33 @@ Section MainTranslation.
           iApply (Hproc with "[Hstk Hu1]").
 
           { 
-            rewrite (stack_free_assertion_trnsl (subst proc_pre subst_map') stk_id' stk_id mp) in Hproc_frame_pre. 2 : { apply stack_free_assertion_subst. destruct Hspec_StackFree as [Hpre_stack_free _]. done. }
-
+            rewrite (stack_free_assertion_trnsl Γ (subst proc_pre subst_map') stk_id' stk_id mp) in Hproc_frame_pre. 2 : { apply stack_free_assertion_subst. destruct Hspec_StackFree as [Hpre_stack_free _]. done. }
 
             iFrame.
-            pose proof (trnsl_assertion_w_lexpr_subst proc_pre lexprs proc_args.*1 arg_vals stk_id mp u1 proc_frame_pre Hlexprs_arg_vals Hproc_pre Hproc_frame_pre) as Himpl.
+            pose proof (trnsl_assertion_w_lexpr_subst Γ proc_pre lexprs proc_args.*1 arg_vals stk_id mp u1 proc_frame_pre Hlexprs_arg_vals Hproc_pre Hproc_frame_pre) as Himpl.
             iApply Himpl. iFrame.
           }
 
           
           iNext. iExact "HΦ".
-
-
           }
 
           {
             iNext. iIntros "[Hstk Hq]".
             iApply "HΦ". iExists (trnsl_val ret_val).
           
-            destruct (trnsl_assertion (subst proc_post (<["#ret_var":=LVar lvar_x]> subst_map)) stk_id
+            destruct (trnsl_assertion Γ (subst proc_post (<["#ret_var":=LVar lvar_x]> subst_map)) stk_id
             (λ x0 : lvar, if (x0 =? lvar_x)%string then trnsl_val ret_val else mp x0)) 
             eqn:Hpost; try done.
             
             iSplitR "Hq". 
             { rewrite fresh_mp_rewrite_symb_stk_to_stk_frm_compat; try done. rewrite trnsl_lval_trnsl_val_inverse. iFrame. } 
             
-            { pose proof (trnsl_assertion_w_lexpr_subst_r proc_post lexprs proc_args.*1 arg_vals lvar_x ret_val stk stk_id mp u proc_frame_post H Hlexprs_arg_vals Hpost Hproc_frame_post) as Himpl. iApply Himpl. iFrame. }
+            { pose proof (trnsl_assertion_w_lexpr_subst_r Γ proc_post lexprs proc_args.*1 arg_vals lvar_x ret_val stk stk_id mp u proc_frame_post H Hlexprs_arg_vals Hpost Hproc_frame_post) as Himpl. iApply Himpl. iFrame. }
             
             
           }
-
         }
-
 
         {   
           (* proc_body != Skip *)
@@ -1035,18 +967,18 @@ Section MainTranslation.
 
         (* destruct HPostCond' as [ret_val HPostCond]. *)
 
-        pose proof (proc_specs_valid proc_name (Proc proc_args proc_locals proc_pre proc_post proc_body) arg_vals ) as [ret_val Hproc]; try done.
+        pose proof (proc_specs_valid Γ proc_name (Proc proc_args proc_locals proc_pre proc_post proc_body) arg_vals ) as [ret_val Hproc]; try done.
 
         set (subst_map' := @list_to_map var LExpr (gmap var LExpr) _ _ (zip (proc_args).*1 (map (λ val, LVal (trnsl_val val)) arg_vals))).
 
-          destruct (trnsl_assertion (subst proc_pre subst_map') stk_id mp) as [ proc_frame_pre |] eqn: Hproc_frame_pre.
+          destruct (trnsl_assertion Γ (subst proc_pre subst_map') stk_id mp) as [ proc_frame_pre |] eqn: Hproc_frame_pre.
           
           2 : {  
             (* trnsl_assertion (subst proc_pre subst_map') stk_id' mp CANNOT BE None *)
             admit.
           }
 
-          destruct (trnsl_assertion (subst proc_post (<["#ret_val":=LVal (trnsl_val ret_val)]> subst_map')) stk_id mp) as [ proc_frame_post |] eqn: Hproc_frame_post.
+          destruct (trnsl_assertion Γ (subst proc_post (<["#ret_val":=LVal (trnsl_val ret_val)]> subst_map')) stk_id mp) as [ proc_frame_post |] eqn: Hproc_frame_post.
 
           2 : {
             (* trnsl_assertion (subst proc_pre subst_map') stk_id' mp CANNOT BE None *)
@@ -1075,9 +1007,9 @@ Section MainTranslation.
 
           simpl in HlocalsDef. pose proof (Hproc HlocalsDef) as Hproc.
 
-          rewrite (stack_free_assertion_trnsl (subst proc_pre subst_map') stk_id stk_id' mp) in Hproc_frame_pre. 2 : { apply stack_free_assertion_subst. destruct Hspec_StackFree; done. }
+          rewrite (stack_free_assertion_trnsl Γ (subst proc_pre subst_map') stk_id stk_id' mp) in Hproc_frame_pre. 2 : { apply stack_free_assertion_subst. destruct Hspec_StackFree; done. }
 
-          rewrite (stack_free_assertion_trnsl (subst proc_post (<["#ret_val":=LVal (trnsl_val ret_val)]> subst_map')) stk_id stk_id' mp) in Hproc_frame_post. 2 : { apply stack_free_assertion_subst. destruct Hspec_StackFree; done. }
+          rewrite (stack_free_assertion_trnsl Γ (subst proc_post (<["#ret_val":=LVal (trnsl_val ret_val)]> subst_map')) stk_id stk_id' mp) in Hproc_frame_post. 2 : { apply stack_free_assertion_subst. destruct Hspec_StackFree; done. }
 
           pose proof (Hproc Hproc_frame_pre Hproc_frame_post) as Hproc.
 
@@ -1096,17 +1028,16 @@ Section MainTranslation.
           iApply (Hproc with "[Hstk Hu1]").
 
           { 
-            rewrite (stack_free_assertion_trnsl (subst proc_pre subst_map') stk_id' stk_id mp) in Hproc_frame_pre. 2 : { apply stack_free_assertion_subst. destruct Hspec_StackFree as [Hpre_stack_free _]. done. }
+            rewrite (stack_free_assertion_trnsl Γ (subst proc_pre subst_map') stk_id' stk_id mp) in Hproc_frame_pre. 2 : { apply stack_free_assertion_subst. destruct Hspec_StackFree as [Hpre_stack_free _]. done. }
 
 
             iFrame.
-            pose proof (trnsl_assertion_w_lexpr_subst proc_pre lexprs proc_args.*1 arg_vals stk_id mp u1 proc_frame_pre Hlexprs_arg_vals Hproc_pre Hproc_frame_pre) as Himpl.
+            pose proof (trnsl_assertion_w_lexpr_subst Γ proc_pre lexprs proc_args.*1 arg_vals stk_id mp u1 proc_frame_pre Hlexprs_arg_vals Hproc_pre Hproc_frame_pre) as Himpl.
             iApply Himpl. iFrame.
           }
 
           
           iNext. iExact "HΦ".
-
 
           }
 
@@ -1114,27 +1045,44 @@ Section MainTranslation.
             iNext. iIntros "[Hstk Hq]".
             iApply "HΦ". iExists (trnsl_val ret_val).
           
-            destruct (trnsl_assertion (subst proc_post (<["#ret_var":=LVar lvar_x]> subst_map)) stk_id
+            destruct (trnsl_assertion Γ (subst proc_post (<["#ret_var":=LVar lvar_x]> subst_map)) stk_id
             (λ x0 : lvar, if (x0 =? lvar_x)%string then trnsl_val ret_val else mp x0)) 
             eqn:Hpost; try done.
             
             iSplitR "Hq". 
             { rewrite fresh_mp_rewrite_symb_stk_to_stk_frm_compat; try done. rewrite trnsl_lval_trnsl_val_inverse. iFrame. } 
             
-            { pose proof (trnsl_assertion_w_lexpr_subst_r proc_post lexprs proc_args.*1 arg_vals lvar_x ret_val stk stk_id mp u proc_frame_post H Hlexprs_arg_vals Hpost Hproc_frame_post) as Himpl. iApply Himpl. iFrame. }
-            
-            
+            { pose proof (trnsl_assertion_w_lexpr_subst_r Γ proc_post lexprs proc_args.*1 arg_vals lvar_x ret_val stk stk_id mp u proc_frame_post H Hlexprs_arg_vals Hpost Hproc_frame_post) as Himpl. iApply Himpl. iFrame. }
           }
 
         }
 
       }
 
+      1 : {
+        (* FPU *)
+        unfold trnsl_hoare_triple; simpl.
+        specialize (RAPack_fpuValid Γ RAPack old_val new_val) as HRA_fpu.
+        destruct (Γ RAPack) as [i [U [Hdisc [Heq_car [Hindx [Hcomp Hval]]]]]].
+
+        iIntros "[Hstack Hown]".
+        iDestruct "Hown" as (l) "[%Heq Hown]".
+
+        iFrame.
+
+        apply (HRA_fpu) in H0.
+
+        iMod (own_update _ 
+          (transport (f_equal cmra_car Hindx) ((transport Heq_car old_val))) 
+          (transport (f_equal cmra_car Hindx) ((transport Heq_car new_val)))
+       with "Hown") as "Hown".
+
+       { apply transport_cmra_update. exact H0.  }
+
+       iModIntro. iExists l. iFrame. iPureIntro. exact Heq.
 
 
-
-
-      
+      }
 
     Admitted.
   
